Show continuitiy of ESem

Denotational-Common.thy
@@ -82,7 +82,9 @@ lemma heapToEnv_cong[fundef_cong]:
 definition heapExtend :: "Env \<Rightarrow> heap \<Rightarrow> (exp \<Rightarrow> Env \<Rightarrow> Value)  \<Rightarrow> (var, Value) fmap"
   where
   "heapExtend \<rho> h eval =
-    (if (\<forall>e \<in> snd ` set h. cont (eval e)) then fmap_update \<rho> (fix1 (fmap_bottom (fst ` set h)) (\<Lambda> \<rho>' . heapToEnv h (\<lambda> e. eval e \<rho>'))) else fempty)"
+    (if (\<forall>e \<in> snd ` set h. cont (eval e))
+    then fmap_update \<rho> (fix1 (fmap_bottom (fst ` set h)) (\<Lambda> \<rho>' . heapToEnv h (\<lambda> e. eval e \<rho>')))
+    else fempty)"
 
 lemma perm_still_cont[simp]: "cont (\<pi> \<bullet> f) = cont (f :: ('a :: cont_pt) \<Rightarrow> ('b :: cont_pt))"
 proof
@@ -155,5 +157,8 @@ lemma heapExtend_cong[fundef_cong]:
   unfolding heapExtend_def
   by (auto cong:heapToEnv_cong)
 
+lemma heapExtend_cont[simp,cont2cont]: "cont (\<lambda>\<rho>. heapExtend \<rho> h eval)"
+  unfolding heapExtend_def
+  by (cases "\<forall> e \<in> snd ` set h.  cont (eval e)", auto)
 
 end
